Proved wpc_RPCClient__MakeRequest with new setup for quiesce_fupd

src/program_proof/lockservice/incr_proof.v
@@ -82,21 +82,24 @@ Proof.
 Qed.
 
 Lemma rpc_atomic_pre_mono_strong cid γrpc P Q :
-  <bdisc> (P -∗ own γrpc.(proc) (Excl ()) ={⊤}=∗ own γrpc.(proc) (Excl ()) ∗ Q) -∗
+  □(P -∗ own γrpc.(proc) (Excl ()) ={⊤}=∗ own γrpc.(proc) (Excl ()) ∗ Q) -∗
   rpc_atomic_pre γrpc cid P -∗
   rpc_atomic_pre γrpc cid Q.
 Proof.
-  iIntros "HPQ HatomicP".
+  iIntros "#HPQ HatomicP".
   iModIntro.
   iIntros (seq) "Hcown".
   iMod ("HatomicP" $! seq with "Hcown") as "[Hcown HatomicP]".
   iFrame.
-  (*
+  unfold laterable.make_laterable.
+  iDestruct "HatomicP" as (R) "[HR #HatomicP]".
+  iExists (R). iFrame.
+  iModIntro.
+  iModIntro.
+  iIntros "HR". iSpecialize ("HatomicP" with "HR").
   iApply (rpc_atomic_pre_fupd_mono_strong with "[HPQ] HatomicP").
   iIntros "HP #Hlb Hγproc". iApply ("HPQ" with "HP Hγproc").
 Qed.
-*)
-Admitted.
 
 (*
 Lemma rpc_atomic_pre_fupd_mono γrpc cid seq P Q:
@@ -124,15 +127,26 @@ Proof.
 Qed.
 *)
 
+Definition quiesce_fupd γrpc cid seqno PreCond PostCond (args:RPCValC) : iProp Σ :=
+  laterable.make_laterable (rpc_atomic_pre_fupd γrpc cid seqno (▷ PreCond args ∨ ▷ ∃ ret:u64, PostCond args ret))%I.
+
+Definition quiesceable_pre γrpc cid (args:RPCValC) PreCond PostCond : iProp Σ :=
+  rpc_atomic_pre γrpc cid (▷ PreCond args ∨ ▷ ∃ ret:u64, PostCond args ret)%I.
+
+Global Instance quiesceable_pre_disc γrpc cid args PreCond PostCond : (Discretizable
+       (quiesceable_pre γrpc cid args PreCond PostCond)).
+Proof.
+  rewrite /Discretizable.
+  by rewrite -own_discrete_idemp.
+Defined.
+
 Lemma quiesce_request (req:RPCRequest) γrpc γreq (PreCond:RPCValC → iProp Σ) PostCond  :
   is_RPCServer γrpc -∗
   is_RPCRequest γrpc γreq PreCond PostCond req -∗
   (RPCRequest_token γreq) -∗
-  rpc_atomic_pre γrpc req.(Req_CID) (▷ PreCond req.(Req_Args) ∨ ▷(∃ ret, PostCond req.(Req_Args) ret)).
+  quiesceable_pre γrpc req.(Req_CID) req.(Req_Args) PreCond PostCond.
 Proof.
     iIntros "#Hsrpc #His_req Hγpost".
-    (* iDestruct (fmcounter_map_get_lb with "Hcown") as "#Hcseq_lb". *)
-    (* iExists (RPCRequest_token γreq). *)
     iFrame "#∗".
 
     iModIntro.
@@ -186,138 +200,14 @@ Proof.
     }
 Qed.
 
-(*
-(* Want resources R in invariant with the property that ▷ R -∗ (rpc_atomic_pre_fupd blah)
-   Want ∃ R, ⌜Timeless(R)⌝ ∗ invariant
- *)
-
-
-Print laterable.make_laterable.
-Search "except_0".
-Search Timeless.
-
-Print inv_def.
-
-Definition tinv {invG0 : invG Σ} (N : namespace) (P : iProp Σ) :=
-  (□ (∀ E : coPset, ⌜↑N ⊆ E⌝ → |0={E,E ∖ ↑N}=> P ∗ (P -∗ |0={E ∖ ↑N,E}=> True)))%I.
-
-Definition latered P : iProp Σ := ∃(Q:iProp Σ), Q ∗ □(▷ Q -∗ ◇P).
-(* Need to have the fmcounter fact because the quiesce_fupd in the
-   quiesceable_pre is specialized to a particular seqno, while we need to know
-   that any seqno is good. The fmcounter fact is one way to get around this.
-   Alternatively, could also maybe make the RPCRequestInvariant contain
-   (quiesce_fupd ∧ quiesceable_pre).
- *)
-
-Definition sem_invariant_try P N :
-  latered P ={⊤}=∗ tinv N (P).
-Proof.
-  iIntros "HP".
-  iDestruct "HP" as (Q) "[HQ #Hwand]".
-  iMod (inv_alloc N ⊤ (Q ∧ ◇ P)%I with "[HQ]") as "#Hinv".
-  {
-    iNext. iSplit.
-    { iFrame. }
-    { iApply "Hwand". iFrame. }
-  }
-  iModIntro.
-  iIntros (E) "!# %HE".
-  iInv "Hinv" as "HN" "HNClose".
-  iLeft in "HN".
-  iDestruct ("Hwand" with "HN") as "HN".
-  iMod "HN".
-  iModIntro.
-  iFrame.
-  iIntros "HP".
-  iMod ("HNClose" with "[HP]").
-  {
-    iNext. iSplit.
-    { admit. } (* This can't work *)
-    iModIntro.
-    iFrame.
-  }
-  done.
-Abort.
-
-Definition tinv_laterable {invG0 : invG Σ} (N : namespace) (P : iProp Σ) :=
-  (□ (∀ E : coPset, ⌜↑N ⊆ E⌝ → |0={E,E ∖ ↑N}=>
-        ∃ Q, (Q ∧ ◇ P) ∗ (Q -∗ |0={E ∖ ↑N,E}=> True)))%I.
-
-Lemma sem_invariant_try P N :
-  latered P ={⊤}=∗ tinv_laterable N (P).
-Proof.
-  iIntros "HP".
-  iDestruct "HP" as (Q) "[HQ #Hwand]".
-  iMod (inv_alloc N ⊤ (Q)%I with "HQ") as "#Hinv".
-
-  iModIntro.
-  iIntros (E) "!# %HE".
-  iInv "Hinv" as "HN" "HNClose".
-  iModIntro.
-  iExists (▷ Q)%I.
-  iSplitL "HN".
-  {
-    iSplit.
-    { iFrame. }
-    iApply "Hwand".
-    iFrame.
-  }
-  iIntros "HQ".
-  iMod ("HNClose" with "HQ").
-  iModIntro.
-  done.
-Qed.
-
-(*
-  Want to have tinv (P ∨ R), where R is timeless and P is laterable.
-  |={E, E∖↑N}=> ∃ Q, ((Q ∧ P) ∨ R) ∗ ((Q ∨ R) -∗ |={E∖↑N,E}=> ⊤)
-
-  |={⊤}=>
-*)
-
-Definition tinv_laterable2 (N : namespace) (P:iProp Σ) (F : iProp Σ → iProp Σ) :=
-  (□ (∀ E : coPset, ⌜↑N ⊆ E⌝ → |0={E,E ∖ ↑N}=>
-        ∃ Q, F(Q ∧ ◇ P) ∗ (F(Q) -∗ |0={E ∖ ↑N,E}=> True)))%I.
-
-Lemma sem_invariant_try2 P R N :
-  (latered P) ∨ R ={⊤}=∗ tinv_laterable2 N P (λ A, A ∨ ▷ R).
-Proof.
-  iIntros "HPR".
-  iDestruct "HPR" as "[HP|HR]".
-  {
-    iDestruct "HP" as (Q) "[HQ #Hwand]".
-    iMod (inv_alloc N ⊤ (Q ∨ R)%I with "[HQ]") as "#Hinv".
-    { iLeft. done. }
-    iModIntro.
-    iIntros (E) "!# %HE".
-    iInv "Hinv" as "HN" "HNClose".
-    iModIntro.
-    iExists (▷ Q)%I.
-    iSplitL "HN".
-    {
-      iDestruct "HN" as "[HQ|HR]".
-      {
-        iLeft. iSplit; first done.
-        iApply "Hwand"; done.
-      }
-      { iRight. iFrame. }
-    }
-    iIntros "HQR".
-    iMod ("HNClose" with "[HQR]") as "$"; last by iModIntro.
-    rewrite later_or.
-    done.
-  }
-Abort.
-*)
-
-Lemma quiesce_idemp_1 γrpc cid seqno R Q Rpost :
+(* TODO: get rid explicitly passing args around everywhere *)
+Lemma quiesce_idemp γrpc cid seqno Q args PreCond PostCond :
   cid fm[[γrpc.(cseq)]]≥ int.nat seqno -∗
-  □(▷Rpost -∗ R) -∗
-  □(▷Q -∗ (rpc_atomic_pre_fupd γrpc cid seqno R)) -∗
-  rpc_atomic_pre γrpc cid (▷ Q ∨ ▷ Rpost) -∗
-  rpc_atomic_pre γrpc cid (▷ R).
+  □(▷Q -∗ (rpc_atomic_pre_fupd γrpc cid seqno (▷ PreCond args ∨ ▷ ∃ ret:u64, PostCond args ret))) -∗
+  quiesceable_pre γrpc cid args (λ _, Q) (PostCond) -∗
+  quiesceable_pre γrpc cid args PreCond PostCond.
 Proof.
-  iIntros "#Hseqno_lb #HwandR #Hwand Hatomic_pre".
+  iIntros "#Hseqno_lb #Hwand Hatomic_pre".
   iModIntro.
   iIntros (seq) "Hcown".
   iDestruct (fmcounter_map_agree_lb with "Hcown Hseqno_lb") as %Hseqno_ineq.
@@ -342,124 +232,69 @@ Proof.
     iMod ("Hfupd" with "Hγproc Hlb_seqno") as "[$ $]".
     by iModIntro.
   }
-  { iSpecialize ("HwandR" with "HRpost"). iModIntro. iFrame. }
+  { iFrame. by iModIntro. }
 Qed.
 
-(*
-Lemma quiesce_idemp_2 γrpc cid seqno R Rpost {H:Timeless R}:
-  cid fm[[γrpc.(cseq)]]≥ int.nat seqno -∗
-  <bdisc> (Rpost -∗ R) -∗
-  rpc_atomic_pre γrpc cid (▷ latered (rpc_atomic_pre_fupd γrpc cid seqno R)) -∗
-  rpc_atomic_pre γrpc cid R.
+Lemma quiesce_intro γrpc cid seqno args PreCond PostCond :
+  PreCond args -∗ (quiesce_fupd γrpc cid seqno PreCond PostCond args).
 Proof.
-  iIntros "#Hseqno_lb Hwand Hatomic_pre".
-  iModIntro.
-  iIntros (seq) "Hcown".
-  iDestruct (fmcounter_map_agree_lb with "Hcown Hseqno_lb") as %Hseqno_ineq.
-
-  iDestruct ("Hatomic_pre" $! seq with "Hcown") as ">[Hcown Hfupd]".
+  iIntros.
+  iExists (PreCond args)%I.
   iFrame.
-  iApply (rpc_atomic_pre_fupd_mono_strong with "[Hwand] Hfupd").
-  iIntros "Hfupd #Hlb Hγproc".
-  iDestruct (fmcounter_map_mono_lb (int.nat seqno) with "Hlb") as "#Hlb_seqno".
-  { lia. }
-  iDestruct "Hfupd" as (P) "[HP #Hfupd]".
-
-  iAssert (□ ▷(P -∗ ◇ rpc_atomic_pre_fupd γrpc cid seqno R) )%I as "#Hfupd2".
-  { iApply later_intuitionistically. done. }
-  iDestruct (later_wand with "Hfupd2") as "Hfupd3".
-  iDestruct ("Hfupd3" with "HP") as "Hatomic_fupd".
-  unfold rpc_atomic_pre_fupd.
-
-  iDestruct (later_wand with "Hatomic_fupd") as "Hatomic_fupd".
-  iAssert
-
-  iMod ("Hfupd" with "Hγproc Hlb_seqno") as "[$ [$|HRpost]]".
-  { by iModIntro. }
-  iApply "Hwand". by iModIntro.
-
-
-
-Lemma quiesce_idemp_2 γrpc cid seqno R Rpost {H:Timeless R}:
-  cid fm[[γrpc.(cseq)]]≥ int.nat seqno -∗
-  <bdisc> (Rpost -∗ R) -∗
-  rpc_atomic_pre γrpc cid ((rpc_atomic_pre_fupd γrpc cid seqno R) ∨ Rpost) -∗
-  rpc_atomic_pre γrpc cid R.
-Proof.
-  iIntros "#Hseqno_lb Hwand Hatomic_pre".
-  Search later.
-  iModIntro.
-  iIntros (seq) "Hcown".
-  iDestruct (fmcounter_map_agree_lb with "Hcown Hseqno_lb") as %Hseqno_ineq.
-
-  iDestruct ("Hatomic_pre" $! seq with "Hcown") as ">[Hcown Hfupd]".
+  iModIntro; iFrame.
+  iIntros.
+  iIntros "Hγproc #Hlb".
   iFrame.
-  iApply (rpc_atomic_pre_fupd_mono_strong with "[Hwand] Hfupd").
-  iIntros "Hfupd #Hlb Hγproc".
-  iDestruct (fmcounter_map_mono_lb (int.nat seqno) with "Hlb") as "#Hlb_seqno".
-  { lia. }
-  iDestruct "Hfupd" as "[Hfupd|HRpost]".
-  {
-    Search "laterable".
-    unfold rpc_atomic_pre_fupd.
-    iDestruct ("Hfupd" with "[Hγproc] [Hlb_seqno]") as "HH".
-    { iNext. done. }
-    { iNext. done. }
-    iModIntro.
-  }
-  { iFrame. iApply "Hwand". by iModIntro. }
+    by iModIntro.
 Qed.
-*)
 
-Definition quiesce_fupd γrpc cid seqno PreCond PostCond (args:RPCValC) : iProp Σ :=
-  laterable.make_laterable (rpc_atomic_pre_fupd γrpc cid seqno (▷ PreCond args ∨ ▷ ∃ ret:u64, PostCond args ret))%I.
+Definition quiesce_fupd_raw γrpc cid seqno PreCond PostCond (args:RPCValC) : iProp Σ :=
+  (rpc_atomic_pre_fupd γrpc cid seqno (▷ PreCond args ∨ ▷ ∃ ret:u64, PostCond args ret))%I.
 
-Definition quiesceable_pre γrpc cid (args:RPCValC) PreCond PostCond : iProp Σ :=
-  rpc_atomic_pre γrpc cid (▷ PreCond args ∨ ▷ ∃ ret:u64, PostCond args ret)%I.
+Lemma quiesceable_pre_instantiate γrpc cid seqno args PreCond PostCond :
+  RPCClient_own γrpc cid seqno -∗
+  quiesceable_pre γrpc cid args PreCond PostCond ={⊤}=∗
+  RPCClient_own γrpc cid seqno ∗
+  (quiesce_fupd γrpc cid seqno PreCond PostCond args).
+Proof.
+  iIntros "Hcrpc Hqpre".
+  iDestruct (own_discrete_elim with "Hqpre") as "Hqpre".
+  iMod ("Hqpre" $! seqno with "Hcrpc") as "[Hcrpc Hfupd]".
+  iModIntro. iFrame.
+Qed.
 
+Print is_rpcHandler.
 Lemma wpc_RPCClient__MakeRequest k (f:goose_lang.val) cl_ptr cid args γrpc (PreCond:RPCValC -> iProp Σ) PostCond {_:Discretizable (PreCond args)} {_:∀ reply, Discretizable (PostCond args reply)}:
-  (∀ seqno, is_rpcHandler f γrpc (quiesce_fupd γrpc cid seqno PreCond PostCond) PostCond) -∗
+  □(∀ seqno Q, (□(Q -∗ quiesce_fupd_raw γrpc cid seqno PreCond PostCond args) -∗ is_rpcHandler f γrpc (λ _, Q) PostCond)) -∗
   {{{
-    PreCond args ∗
+    quiesceable_pre γrpc cid args PreCond PostCond ∗
     own_rpcclient cl_ptr γrpc cid ∗
     is_RPCServer γrpc
   }}}
     RPCClient__MakeRequest #cl_ptr f (into_val.to_val args) @ k ; ⊤
-  {{{ (retv:u64), RET #retv; own_rpcclient cl_ptr γrpc cid ∗ PostCond args retv }}}
+  {{{ (retv:u64), RET #retv; own_rpcclient cl_ptr γrpc cid ∗ ▷ PostCond args retv }}}
   {{{ quiesceable_pre γrpc cid args PreCond PostCond }}}.
 Proof using Type*.
-  iIntros "#Hfspec" (Φ Φc) "!# [Hprecond [Hclerk #Hlinv]] HΦ".
+  iIntros "#Hfspec" (Φ Φc) "!# [Hpre [Hclerk #Hlinv]] HΦ".
   iNamed "Hclerk".
 
-  iCache with "Hprecond HΦ".
+  Opaque quiesceable_pre.
+  iCache with "Hpre HΦ".
   { (* Use PreCond to show idemp_fupd *)
     iDestruct "HΦ" as "[HΦc _]".
     iModIntro.
     iApply "HΦc".
-    iModIntro.
-    iIntros.
-    iModIntro.
     iFrame.
-    iIntros.
-    iExists (PreCond args)%I.
-    iFrame.
-    iModIntro; iFrame.
-    iIntros.
-    iIntros "Hγproc #Hlb".
-    iFrame.
-    by iModIntro.
   }
   wpc_rec _.
   { iFromCache. }
 
-  iCache with "Hprecond HΦ".
-  { (* Use PreCond to show idemp_fupd *)
-    (* repeat crash proof *)
+  iCache with "Hpre HΦ".
+  { (* repeat crash proof *)
     iDestruct "HΦ" as "[HΦc _]".
-    iModIntro. iApply "HΦc".
-    iModIntro. iIntros.
-    iModIntro. iFrame.
-    iIntros. admit.
+    iModIntro.
+    iApply "HΦc".
+    iFrame.
   }
   wpc_pures.
   wpc_loadField.
@@ -495,21 +330,10 @@ Proof using Type*.
   iNamed 1.
   wpc_pures.
   iDestruct (fmcounter_map_get_lb with "Hcrpc") as "#Hcseqno_lb". (* Need this to apply quiesce_idemp_1 *)
-  iAssert (quiesce_fupd γrpc cid cseqno PreCond PostCond args)%I with "[Hprecond]" as "Hq".
-  { (* TODO: Use lemma for Precond -> quiesce_fupd PreCond *)
-    iExists (PreCond args)%I.
-    iFrame.
-    iModIntro; iFrame.
-    iIntros.
-    iIntros "Hγproc #Hlb".
-    iFrame.
-    by iModIntro.
-  }
-  unfold quiesce_fupd.
-  unfold laterable.make_laterable.
-  iDestruct "Hq" as (Q) "[HQ #Hwand]".
+  iMod (quiesceable_pre_instantiate with "Hcrpc Hpre") as "[Hcrpc Hqfupd]".
+  unfold quiesce_fupd, laterable.make_laterable.
+  iDestruct "Hqfupd" as (Q) "[HQ #Hqwand]".
   iMod (make_request {| Req_Args:=args; Req_CID:=cid; Req_Seq:=cseqno|} (λ _, Q) PostCond with "[Hlinv] [Hcrpc] [HQ]") as "[Hcseq_own HallocPost]"; eauto.
-  (* { admit. (* TODO: add assumption *) } *)
   { simpl. word. }
   iDestruct "HallocPost" as (γP) "[#Hreqinv_init HγP]".
   (* Prepare the loop invariant *)
@@ -526,20 +350,8 @@ Proof using Type*.
     iDestruct "HΦ" as "[HΦc _]".
     iModIntro.
     iApply "HΦc".
-    simpl.
     iDestruct (quiesce_request with "Hlinv Hreqinv_init HγP") as "Hquiesce_req".
-    simpl.
-    iDestruct (quiesce_idemp_1 γrpc cid _ _ Q (∃ ret : u64, PostCond args ret)%I with "[] [] [Hwand] Hquiesce_req") as "HH".
-    { simpl. iFrame "#". }
-    { iModIntro. admit. (* timeless postcond *) }
-    { admit. (* timeless postcond *) }
-    unfold quiesceable_pre.
-    iRevert "HH".
-    iApply (rpc_atomic_pre_mono_strong).
-    iModIntro.
-    iIntros.
-    iModIntro.
-    iFrame.
+    iDestruct (quiesce_idemp γrpc cid with "Hcseqno_lb Hqwand Hquiesce_req") as "$".
   }
   {
     iIntros "!# __CTX"; iNamed "__CTX".
@@ -548,15 +360,20 @@ Proof using Type*.
     {
       iDestruct "HΦ" as "[HΦc _]".
       iModIntro. iApply "HΦc".
-      iDestruct (quiesce_request with "Hlinv Hreqinv_init HγP") as "Hq".
-      admit. (* repeat above *)
+      iDestruct (quiesce_request with "Hlinv Hreqinv_init HγP") as "Hquiesce_req".
+      iDestruct (quiesce_idemp γrpc cid with "Hcseqno_lb Hqwand Hquiesce_req") as "$".
     }
 
     iDestruct "Hreply" as (reply') "Hreply".
     wpc_pures.
     wpc_bind (RemoteProcedureCall _ _ _). wpc_frame.
     wp_apply (RemoteProcedureCall_spec with "[] [Hreply]").
-    { iSpecialize ("Hfspec" $! cseqno). iFrame "Hfspec". }
+    { iSpecialize ("Hfspec" $! cseqno Q with "[Hqwand]").
+      { iModIntro. iIntros "HQ".
+        iSpecialize ("Hqwand" with "HQ").
+        iFrame.
+      }
+      iFrame "Hfspec". }
     {
       iSplit; last first.
       { unfold read_request.
@@ -565,7 +382,6 @@ Proof using Type*.
         iFrame "Hreply".
         simpl. iPureIntro. lia.
       }
-      (*
       iFrame "Hreqinv_init".
     }
     iIntros (v) "Hrpc_post". iNamed 1.
@@ -622,10 +438,8 @@ Proof using Type*.
     {
       iLeft in "HΦ". iModIntro.
       iApply "HΦ".
-      iDestruct (quiesce_request with "Hlinv Hreqinv_init HγP") as "Hq".
-      iDestruct (quiesce_idemp_1 with "[] Hq") as "Hq".
-      { simpl. iFrame "#". }
-      iFrame.
+      iDestruct (quiesce_request with "Hlinv Hreqinv_init HγP") as "Hquiesce_req".
+      iDestruct (quiesce_idemp γrpc cid with "Hcseqno_lb Hqwand Hquiesce_req") as "$".
     }
 
     wpc_pures.
@@ -640,8 +454,6 @@ Proof using Type*.
 
     iMod (get_request_post with "Hreqinv_init Hrcptstoro HγP") as "HP"; first done.
     simpl.
-    assert (Timeless (PostCond args reply.(Rep_Ret))) by admit. (* Timeless post *)
-    iMod "HP".
     iModIntro.
     iRight in "HΦ".
     iApply "HΦ".
@@ -649,28 +461,14 @@ Proof using Type*.
     iExists _; iFrame.
     iPureIntro.
     word.
-*)
-Admitted.
+  }
+Qed.
 End rpc_proof.
 
 Section kv_proof.
 Context `{!heapG Σ}.
 Context `{!kvserviceG Σ}.
 Variable γ:kvservice_names.
-
-Global Instance quiesceable_pre_disc cid key old_v : (Discretizable
-       (quiesceable_pre γ.(ks_rpcGN) cid (key, (U64 0, ())) (Get_Pre γ old_v) (Get_Post γ old_v))).
-Proof.
-  rewrite /Discretizable.
-  by rewrite -own_discrete_idemp.
-Defined.
-
-Global Instance quiesceable_put_disc cid args : (Discretizable
-       (quiesceable_pre γ.(ks_rpcGN) cid args (Put_Pre γ) (Put_Post γ))).
-Proof.
-  rewrite /Discretizable.
-  by rewrite -own_discrete_idemp.
-Defined.
 
 Definition own_kvclerk γ ck_ptr srv cid : iProp Σ :=
   ∃ (cl_ptr:loc),
